\documentclass{article}
\input{includes}
\usepackage{macros}

\title{2MMR40}
\author{Cor de Leeuw \\
Eindhoven University of Technology
}
\date{\today}

\begin{document}

\maketitle

% \section{Introduction}

\input{preliminaries}

\section{Model}

% Let $N \in \bN$ be the number of neurons.
% Define the drift-generator $L_D^{N} : C^1(\potspace^N) \cap C_0(\potspace^N) \to M_b(\potspace^N)$ as
% % \begin{equation}
% %     L^{\lambda, N}\varphi (\bm{x}) \coloneqq \sum_{i=1}^N b(x^i) \partial_{x^i} \varphi(\bm{x})
% %     + \sum_{i=1}^N \int_\potspace \sbr{\varphi(x^1, \dots, x^{i-1}, y, x^{i+1}, \dots, x^N) - \varphi(\bm{x})} \lambda \kappa(x^i, \bm{x}, \odif{y})
% % \end{equation}
% \begin{equation}
%     L_D^{N}\varphi \coloneqq \bm{b} \cdot \nabla_{\bm{x}} \varphi,
% \end{equation}
% where $\bm{b} : \potspace^N \to \bR^N$ is defined as $\bm{b}(\bm{x}) \coloneqq (b(x^1), \dots, b(x^N))^\top$, where $b \in M_b(\potspace)$ is the physical driving force.
% % but then multiplied with $\1_{(-\infty,V_F)}$.
% % We will assume that $b$ satisfies the following linear growth assumption:
% % \begin{equation}
% %     \forall x \in \potspace : \abs{b(x)} \leq C (1 + \abs{x}),
% % \end{equation}
% % for some constant $C > 0$.
% Note that, in particular, $b$ is locally bounded.
% \newline
% A typical example of such a driving force is the time-homogeneous \textit{leaky model}:
% \begin{equation}
%     b_{\mathrm{leaky}}(x) \coloneqq -(x - V_\mathrm{rest}),
% \end{equation}
% where $V_\mathrm{rest} \in (V_R, V_F)$ is the equilibrium potential.

\input{drift}


\input{jump}





% {\Large Insert MP justification / equivalent SDE}

% We introduce the following SDE
% \begin{equation}
%     \bm{X}_t = \bm{X}_0 + \int_0^t \bm{b}(\bm{X}_{r-}) \odif{r} + \sum
% \end{equation}

% \dots

% Following Theorem 5.13 from \cite{klebaner_introduction_2012}, we can equate the weak solutions of this SDE to the solutions of the \textit{martingale problem}.

% \dots

% If we assume $\omega^{ij} = \omega / N$, and for $\varphi = \frac{1}{N} \bigoplus_i \psi$, the non-spike jump part simplifies to
% \begin{equation}
%     \lambda \int \partial_x \psi (x) \omega \mu_r^\lambda([V_F, \infty)) \mu_r(\odif{x})
% \end{equation}


\input{full generator}



\section{Connection to empirical measure}

\noindent For \(\psi \in C^1(\potspace)\), we now define
\begin{equation}\label{eq:hat-M-derivation-start}
\begin{split}
    \widehat{M}_t^{\lambda, N}[\psi] \coloneqq
    M_t^{\lambda, N}\sbr*{\frac{1}{N} \bigoplus_{i=1}^N \psi}
    &= \frac{1}{N} \sum_{i=1}^N \psi(X_t^i) - \frac{1}{N} \sum_{i=1}^N \psi(X_0^i) - \int_0^t L^{\lambda, N} \br*{\frac{1}{N}\bigoplus_{i=1}^N \psi} (\bm{X}_r) \odif{r} \\
    &= \int_\potspace \psi \odif{\mu_t^{\lambda, N}} - \int_\potspace \psi \odif{\mu_0^{\lambda, N}}
    - \int_0^t \sum_{i=1}^N b(X_{r}^i) \cdot \frac{1}{N} \partial_{x} \psi(X_{r}^i) \odif{r} \\
    % &\quad - \int_0^t \sum_{i=1}^N \int_\potspace \frac{1}{N} \br*{ \psi(y) + \sum_{\substack{j=1 \\ j \neq i}}^N \psi(X_{r}^j) - \sum_{j=1}^N \psi(X_{r}^j) } \lambda \kappa(X_{r}^i, \bm{X}_r, \odif{y}) \odif{r} \\
    &\quad - \int_0^t \int_{\potspace^N} \frac{1}{N} \sum_{i=1}^N \br*{ \psi(y^i) - \psi(X_{r}^i) } \lambda \kappa(\bm{X}_r, \odif{\bm{y}}) \odif{r} \\
    &= \int_\potspace \psi \odif{\mu_t^{\lambda, N}} - \int_\potspace \psi \odif{\mu_0^{\lambda, N}}
    - \int_0^t \int_\potspace b(x) \partial_{x} \psi(x) \mu_r^{\lambda, N}(\odif{x}) \odif{r} \\
    &\quad - \int_0^t \int_{\potspace^N} \frac{1}{N} \sum_{i=1}^N \br*{ \psi(y^i) - \psi(X_{r}^i) } \lambda \kappa(\bm{X}_r, \odif{\bm{y}}) \odif{r} \\
    %
    % &= \frac{1}{N} \sum_{i=1}^N \psi(X_t^i) - \frac{1}{N} \sum_{i=1}^N \psi(X_0^i) \\
    % &\quad - \int_0^t \frac{1}{N} \sum_{i=1}^N \br*{ b(X_{r}^i) \partial_{x} \psi(X_{r}^i) - \int_\potspace \br*{ \psi(y) - \psi(X_{r}^i) } \lambda \kappa(X_{r}^i, \bm{X}_r, \odif{y}) } \odif{r}
\end{split}
\end{equation}
Here we used the empirical measure $\mu^{\lambda,N}$, which is defined as
\begin{equation}
    \br{ t \mapsto \mu_t^{\lambda, N} \coloneqq \Theta_N(\bm{X})_t = \frac{1}{N} \sum_{i=1}^N \delta_{X_t^i} } \in D_{\cP(\potspace)}[0,T]
\end{equation}
where
\begin{equation}
    \Theta_N : D_{\potspace^N}[0,T] \to D_{\cP(\potspace)}[0,T]; (x_\cdot^1,\dots,x_\cdot^N) \mapsto \frac{1}{N} \sum_{i=1}^N \delta_{x_\cdot^i}.
\end{equation}
If we assume $\omega^{ij} = \frac{\omega}{N}$, we get
\begin{equation}\label{eq:kappa-to-mean-kappa}
\begin{split}
    % &\frac{1}{N} \sum_{i=1}^N \int_\potspace \br*{ \psi(y) - \psi(X_{r}^i) } \lambda \kappa(X_{r}^i, \bm{X}_r, \odif{y}) \\
    % &= \frac{1}{N} \sum_{i=1}^N \int_\potspace \br*{ \psi(y) - \psi(X_{r}^i) } \lambda \br{ \indE{[V_F,+\infty)}(X_{r}^i) \delta_{V_R}(\odif{y}) + \indE{(-\infty,V_F)}(X_{r}^i) \delta_{X_{r}^i + \sum_{j=1}^N \omega^{ij} \indE{[V_F,+\infty)}(X_{r}^j)}(\odif{y}) } \\
    % &= \frac{\lambda}{N} \sum_{i=1}^N \br*{ \br*{ \psi(V_R) - \psi(X_{r}^i) } \indE{[V_F,+\infty)}(X_{r}^i)
    % + \br*{ \psi(X_{r}^i + \frac{1}{N} \sum_{j=1}^N \omega \indE{[V_F,+\infty)}(X_{r}^j)) - \psi(X_{r}^i) } \indE{(-\infty,V_F)}(X_{r}^i) } \\
    % &= \frac{\lambda}{N} \sum_{i=1}^N \br*{ \br*{ \psi(V_R) - \psi(X_{r}^i) } \indE{[V_F,+\infty)}(X_{r}^i)
    % + \br*{ \psi(X_{r}^i + \omega \mu_r^{\lambda, N}([V_F,+\infty))) - \psi(X_{r}^i) } \indE{(-\infty,V_F)}(X_{r}^i) } \\
    % &= \lambda \int_\potspace \br*{ \br*{ \psi(V_R) - \psi(x) } \indE{[V_F,+\infty)}(x)
    % + \br*{ \psi(x + \omega \mu_r^{\lambda, N}([V_F,+\infty))) - \psi(x) } \indE{(-\infty,V_F)}(x) } \mu_{r}^{\lambda, N}(\odif{x}) \\
    % &= \int_\potspace \int_\potspace (\psi(y) - \psi(x)) \lambda \ol{\kappa}_r(x, \odif{y}) \mu_{r}^{\lambda, N}(\odif{x}).
    %
    % \frac{1}{N} \kappa(\bm{X}_r,\odif{\bm{y}}) &= \frac{1}{N}\sum_{i=1}^N \delta_{\bm{\jtarg}^i(\bm{X}_r)}(\odif{\bm{y}}) \\
    % &?=? \int_\potspace \underbrace{\br*{ \indE{[V_F,+\infty)}(x) \delta_{V_R}(\odif{y^i}) + \indE{(-\infty,V_F)}(x) \delta_{x + \omega \mu_r^{\lambda, N}([V_F,+\infty))}(\odif{y^i}) }}_{\eqqcolon \ol{\kappa}_r(x, \odif{y^i})} \mu_{r}^{\lambda, N}(\odif{x})
    %
    &\int_{\potspace^N} \frac{1}{N} \sum_{j=1}^N \br*{ \psi(y^j) - \psi(X_{r}^j) } \lambda \kappa(\bm{X}_r, \odif{\bm{y}}) \\
    &= \frac{\lambda}{N} \sum_{j=1}^N \int_{\potspace^N} \br*{ \psi(y^j) - \psi(X_{r}^j) } \sum_{i=1}^N \delta_{\bm{\jtarg}^i(\bm{X}_r)}(\odif{\bm{y}}) \\
    &= \frac{\lambda}{N} \sum_{j=1}^N \sum_{i=1}^N \int_{\potspace^N} \br*{ \psi(y^j) - \psi(X_{r}^j) } \delta_{\jtarg^i(\bm{X}_r)}(\odif{y^i}) \prod_{k \neq i} \delta_{X_r^k}(\odif{y^k}) \\
    &= \frac{\lambda}{N} \sum_{j=1}^N \sum_{i=1}^N \br{ \br*{ \psi(\jtarg^i(\bm{X}_r)) - \psi(X_{r}^j) } \ind{i = j} + (0 - 0) \ind{i \neq j} } \\
    &= \frac{\lambda}{N} \sum_{i=1}^N \br*{ \psi(\jtarg^i(\bm{X}_r)) - \psi(X_{r}^j) } \\
    &= \frac{\lambda}{N} \sum_{i=1}^N \br*{ \br*{ \psi(V_R) - \psi(X_{r}^i) } \indE{[V_F,+\infty)}(X_{r}^i)
    + \br*{ \psi(X_{r}^i + \frac{\omega}{N} \sum_{j=1}^N \indE{[V_F,+\infty)}(X_{r}^j)) - \psi(X_{r}^i) } \indE{(-\infty,V_F)}(X_{r}^i) } \\
    &= \lambda \int_\potspace \br*{ \br*{ \psi(V_R) - \psi(x) } \indE{[V_F,+\infty)}(x)
    + \br*{ \psi(x + \omega \mu_r^{\lambda, N}([V_F,+\infty))) - \psi(x) } \indE{(-\infty,V_F)}(x) } \mu_{r}^{\lambda, N}(\odif{x}) \\
    &= \int_\potspace \int_\potspace (\psi(y) - \psi(x)) \lambda \ol{\kappa}_r(x, \odif{y}) \mu_{r}^{\lambda, N}(\odif{x})
\end{split}
\end{equation}
for
\begin{equation}
    \ol{\kappa}_r(x, \odif{y}) \coloneqq \delta_{\bar{\jtarg}_r(x)}(\odif{y}),
    \quad\text{and}\quad
    \ol{\jtarg}_r(x) \coloneqq \begin{cases}
        x + \omega \mu_r^{\lambda, N}([V_F,+\infty)) &\text{if } x < V_F, \\
        V_R &\text{if } x \geq V_F.
    \end{cases}
\end{equation}
Substituting this into \zcref{eq:hat-M-derivation-start} yields
\begin{equation}
\begin{split}
    \widehat{M}_t^{\lambda, N}[\psi]
    % &= \frac{1}{N} \sum_{i=1}^N \psi(X_t^i) - \frac{1}{N} \sum_{i=1}^N \psi(X_0^i) - \int_0^t \frac{1}{N} \sum_{i=1}^N b(X_{r}^i) \partial_{x} \psi(X_{r}^i) \odif{r} \\
    % &\quad - \lambda \int_0^t \frac{1}{N} \sum_{i=1}^N \sbr*{ \br*{ \psi(V_F) - \psi(X_{r}^i) } \indE{[V_F,+\infty)}(X_{r}^i)
    % + \br*{ \psi(X_{r}^i + \omega \mu_r^{\lambda, N}([V_F,+\infty))) - \psi(X_{r}^i) } \indE{(-\infty,V_F)}(X_{r}^i) } \odif{r} \\
    % &= \int_\potspace \psi \odif{\mu_t^{\lambda, N}} - \int_\potspace \psi \odif{\mu_0^{\lambda, N}} - \int_0^t \int_\potspace b(x) \partial_x \psi(x) \mu_{r}^{\lambda, N}(\odif{x}) \odif{r}\\
    % &\quad - \lambda \int_0^t \br*{ \int_{-\infty}^{V_F} \br*{ \psi(x + \omega \mu_r^{\lambda, N}([V_F,+\infty))) - \psi(x) } \mu_{r}^{\lambda, N}(\odif{x}) + \int_{V_F}^\infty (\psi(V_F) - \psi(x)) \mu_{r}^{\lambda, N}(\odif{x}) } \\
    %
    &= \int_\potspace \psi \odif{\mu_t^{\lambda, N}} - \int_\potspace \psi \odif{\mu_0^{\lambda, N}}
    - \int_0^t \int_\potspace \underbrace{\br*{ b(x) \partial_x \psi(x) + \int_\potspace (\psi(y) - \psi(x)) \lambda \ol{\kappa}_r(x, \odif{y}) }}_{\eqqcolon \widehat{L}_r^{\lambda, N} [\psi](x)} \mu_{r}^{\lambda, N}(\odif{x}) \odif{r}.
\end{split}
\end{equation}
Note that this can also be interpreted as a random variable in $\mu^{\lambda,N}$ instead of $\bm{X}$, where $\widehat{L}_r^{\lambda, N}$ also depends on the empirical measure through $\ol{\kappa}$.

\bigskip

The law of $(\mu_t^{\lambda, N})_{t\in[0,T]}$ is given by
\begin{equation}
    \lawmu^{\lambda,N} \coloneqq \Theta_N \# P^{\lambda, N} = P^{\lambda, N} \circ \Theta_N^{-1} \in \cP(D_{\cP(\potspace)}[0,T]),
\end{equation}
which is defined on the $\sigma$-algebra
\begin{equation}
    \widehat{\cF} \coloneqq \Theta_N \# \cF \coloneqq \{B \subseteq D_{\cP(\potspace)}[0,T] : \Theta_N^{-1}(B) \in \cF\}.
\end{equation}

\begin{corollary}\label{cor:hat-M-mart}
    $\widehat{M}_t^{\lambda, N}[\psi]$ is a martingale on $(D_{\cP(\potspace)}[0,T], \widehat{\cF}, \lawmu^{\lambda,N})$ adapted to the filtration $\widehat{\cF}_t \coloneqq \Theta_N \# \cF_t$.
\end{corollary}
\begin{proof}
    Adaptation and integrability are clear from \zcref{thm:mart-problem-sol}.
    For $s > t$, $B \in \widehat{\cF}_t$,
    \begin{equation}
    \begin{split}
        \int_B \widehat{M}_{s}^{\lambda, N}[\psi] \odif{\lawmu^{\lambda,N}}
        &= \int_B \sbr*{ \int_\potspace \psi \odif{\nu_s} - \int_\potspace \psi \odif{\nu_0} - \int_0^s \int_\potspace \widehat{L}_r^{\lambda, N} [\psi](x) \nu_{r}(\odif{x}) \odif{r} } \lawmu^{\lambda,N} (\odif{\nu}) \\
        &= \int_{\Theta_N(\Theta_N^{-1}(B))} \sbr*{ \int_\potspace \psi \odif{\nu_s} - \int_\potspace \psi \odif{\nu_0} - \int_0^s \int_\potspace \widehat{L}_r^{\lambda, N} [\psi](x) \nu_{r}(\odif{x}) \odif{r} } \Theta_N \# P^{\lambda, N} (\odif{\nu}) \\
        &= \int_{\Theta_N^{-1}(B)} \sbr*{ \int_\potspace \psi(x) (\Theta_N(\omega))_s(\odif{x}) - \int_\potspace \psi(x) (\Theta_N(\omega))_0(\odif{x}) - \int_0^s \int_\potspace \widehat{L}_r^{\lambda, N} [\psi](x) (\Theta_N(\omega))_{r}(\odif{x}) \odif{r} } P^{\lambda, N} (\odif{\omega}) \\
        &= \int_{\Theta_N^{-1}(B)} \sbr*{ \int_\potspace \psi(x) \mu_s^{\lambda,N}(\odif{x}) - \int_\potspace \psi(x) \mu_0^{\lambda,N}(\odif{x}) - \int_0^s \int_\potspace \widehat{L}_r^{\lambda, N} [\psi](x) \mu_{r}^{\lambda,N}(\odif{x}) \odif{r} } \odif{P^{\lambda, N}} \\
        &= \int_{\Theta_N^{-1}(B)} \widehat{M}_s^{\lambda, N}[\psi] \odif{P^{\lambda, N}} \\
        &= \int_{\Theta_N^{-1}(B)} \widehat{M}_t^{\lambda, N}[\psi] \odif{P^{\lambda, N}}
        = \int_B \widehat{M}_t^{\lambda, N}[\psi] \odif{\lawmu^{\lambda,N}},
    \end{split}
    \end{equation}
    which implies that
    \begin{equation}
        \Exp{\lawmu^{\lambda,N}}{\widehat{M}_{s}^{\lambda, N}[\psi] \given \widehat{\cF}_t} = \widehat{M}_t^{\lambda, N}[\psi].
    \end{equation}
\end{proof}


If $(\mu_t^{\lambda, N})_{t\in[0,T]}$ would converge a.s. for $N\to\infty$ w.r.t. Skorokhod topology, it would follow by Proposition 5.2 (EK) that it would converge pointwise at continuity points.
This would make $\widehat{M}_t^{\lambda, N}[\psi]$ converge too.
But unfortunately this will not apply; at most $(\lawmu^{\lambda,N})$ will converge narrowly due to being tight.


\section{Vanishing variance}

Instead, we will show that the variance of $(\widehat{M}_t^{\lambda,N}[\psi])_{t\in[0,T]}$ vanishes for large $N$, implying that it has a deterministic limit.
In the following, we suppress the dependence on $\psi$.

\begin{proposition}\label{prop:vanishing-variance}  % could remove variance, and just show quad. var. goes to zero as that is all I need, right?
For all $\lambda > 0$, $t \in [0,T]$,
\begin{equation}
    \lim_{N\to\infty} \Var{\lawmu^{\lambda,N}}{\widehat{M}_t^{\lambda,N}} = 0.
\end{equation}
\end{proposition}
\begin{proof}
Recall that $(\widehat{M}_s^{\lambda,N})_{s\in[0,T]}$ is a martingale by \zcref{cor:hat-M-mart}.
In particular,
\begin{equation}
    \Exp{\lawmu^{\lambda,N}}{\widehat{M}_t^{\lambda,N}} = \Exp{\lawmu^{\lambda,N}}{\widehat{M}_0^{\lambda,N}}
    \overset{\zcref{eq:M-def}}{=} \Exp{\lawmu^{\lambda,N}}{0} = 0.
\end{equation}
Note also that $(\widehat{M}_s^{\lambda,N})_{s\in[0,T]}$ is bounded, so in particular square integrable.
Hence the variance exists and equals the second moment.
We can relate the second moment to the expectation of the quadratic variation, for which we write $\sbr{\widehat{M}^{\lambda,N}}_t$, using Theorem 7.27 from \cite[201]{klebaner_introduction_2012}.
Namely, since $\widehat{M}_0^{\lambda,N} = 0$,
\begin{equation}
    \Exp{\lawmu^{\lambda,N}}{(\widehat{M}_t^{\lambda,N})^2} = \Exp{\lawmu^{\lambda,N}}{\sbr{\widehat{M}^{\lambda,N}}_t}.
\end{equation}
% \begin{equation}
%     (\widehat{M}_t^{\lambda,N})^2 = \abr{\widehat{M}^{\lambda,N}}_t + 2 \int_0^t \widehat{M}_{s-}^{\lambda,N} \odif{\widehat{M}_s^{\lambda,N}}
% \end{equation}
% Note that $(\widehat{M}_s^{\lambda,N})_{s\in[0,T]}$ is càdlàg by \zcref{eq:M-def} and adapted, so $(\widehat{M}_{s-}^{\lambda,N})_{s\in[0,T]}$ is left-continuous and adapted.
% This means that it is predictable (see e.g. Definition 8.3 \cite{klebaner_introduction_2012}), so as $(\widehat{M}_s^{\lambda,N})_{s\in[0,T]}$ is bounded the stochastic integral is well-defined.

Now denote
\begin{equation}\label{eq:M=S-A}
    \widehat{M}_t^{\lambda,N} = \int_\potspace \psi \odif{\mu_t^{\lambda, N}} - \int_\potspace \psi \odif{\mu_0^{\lambda, N}} - \int_0^t \int_\potspace \widehat{L}_r^{\lambda, N} [\psi](x) \mu_{r}^{\lambda, N}(\odif{x}) \odif{r}
    \eqqcolon S_t - S_0 - A_t,
\end{equation}
where $(S_r)_{r\in[0,T]}$ is a semimartingale and $(A_r)_{r\in[0,T]}$ a process of bounded variation.
Then by Itô's formula for semimartingales ((8.58) in \cite[236]{klebaner_introduction_2012}, with $f(x) \coloneqq x^2$) we have
\begin{equation}\label{eq:S^2-q-var-rel}
\begin{split}
    S_t^2 - S_0^2
    &= 2 \int_0^t S_{r-} \odif{S_r} + \int_0^t \odif{\sbr{S}_r^c}
    + \sum_{r \leq t} \br{ S_r^2 - S_{r-}^2  - 2 S_{r-} (S_r - S_{r-}) } \\
    &= 2 \int_0^t S_{r-} \odif{S_r} + \sbr{S}_t^c
    + \sum_{r \leq t} \br{ S_r - S_{r-} }^2 \\
    &= 2 \int_0^t S_{r-} \odif{S_r} + \sbr{S}_t.
\end{split}
\end{equation}

By choosing $\varphi \coloneqq \br{ \frac{1}{N} \bigoplus_{i=1}^N \psi }^2$ in \zcref{eq:M-def}, we get
\begin{equation}
\begin{split}
    M_t^{\lambda, N}\sbr*{ \br*{ \frac{1}{N} \bigoplus_{i=1}^N \psi }^2 }
    &= \br*{\frac{1}{N} \sum_{i=1}^N \psi(X_t^i)}^2 - \br*{\frac{1}{N} \sum_{i=1}^N \psi(X_0^i)}^2
    - \int_0^t L^{\lambda, N}(\br*{ \frac{1}{N} \bigoplus_{i=1}^N \psi }^2) (\bm{X}_r) \odif{r} \\
    %
    &= \br*{ \int_\potspace \psi(x) \mu_t^{\lambda, N}(\odif{x}) }^2 - \br*{ \int_\potspace \psi(x) \mu_0^{\lambda, N}(\odif{x}) }^2 \\
    &\quad {} - \int_0^t \Bigg\{ \sum_{i=1}^N b(X_r^i) \partial_{x^i}\br*{ \frac{1}{N} \bigoplus_{i=1}^N \psi }^2 (\bm{X}_r) \\
    &\quad {} + \sum_{i=1}^N \int_\potspace \sbr*{  \frac{1}{N^2} \br*{ \sum_{\substack{j=1 \\ j \neq i}}^N \psi(X_r^j) + \psi(y) }^2 - \frac{1}{N^2} \br*{ \sum_{j=1}^N \psi(X_r^j) }^2 } \lambda \kappa(X_r^i,\bm{X}_r,\odif{y}) \Bigg\} \odif{r} \\
    %
    &= \br*{ \int_\potspace \psi(x) \mu_t^{\lambda, N}(\odif{x}) }^2 - \br*{ \int_\potspace \psi(x) \mu_0^{\lambda, N}(\odif{x}) }^2 \\
    &\quad {} - \int_0^t \Bigg\{ \frac{1}{N^2} \sum_{i=1}^N b(X_r^i) \cdot 2 \br*{ \sum_{j=1}^N \psi(X_r^j) } \cdot \partial_x \psi(X_r^i) \\
    &\quad + \frac{1}{N^2} \sum_{i=1}^N \int_\potspace \sbr*{ \br*{ \sum_{\substack{j=1 \\ j \neq i}}^N \psi(X_r^j) }^2 + 2 \psi(y) \sum_{\substack{j=1 \\ j \neq i}}^N \psi(X_r^i) + \psi^2(y) - \br*{ \sum_{j=1}^N \psi(X_r^j) }^2 } \lambda \kappa(X_r^i,\bm{X}_r,\odif{y}) \Bigg\} \odif{r} \\
    %
    &= \br*{ \int_\potspace \psi(x) \mu_t^{\lambda, N}(\odif{x}) }^2 - \br*{ \int_\potspace \psi(x) \mu_0^{\lambda, N}(\odif{x}) }^2 \\
    &\quad {} - \int_0^t \Bigg\{ 2 \int_\potspace \int_\potspace b(x) \psi(y) \partial_x \psi (x) \mu_r^{\lambda,N}(\odif{x}) \mu_r^{\lambda,N}(\odif{y}) \\
    &\quad + \frac{1}{N^2} \sum_{i=1}^N \int_\potspace \sbr*{ 2 \br*{\sum_{\substack{j=1 \\ j \neq i}}^N \psi(X_r^j)} (\psi(y) - \psi(X_r^i)) + \psi^2(y) - \psi^2(X_r^i) } \lambda \kappa(X_r^i,\bm{X}_r,\odif{y}) \Bigg\} \odif{r} \\
    %
    % &= \br*{ \int_\potspace \psi(x) \mu_t^{\lambda, N}(\odif{x}) }^2 - \br*{ \int_\potspace \psi(x) \mu_0^{\lambda, N}(\odif{x}) }^2 \\
    % &\quad {} - \int_0^t \Bigg\{ 2 \int_\potspace \int_\potspace b(x) \psi(y) \partial_x \psi (x) \mu_r^{\lambda,N}(\odif{x}) \mu_r^{\lambda,N}(\odif{y}) \\
    % &\quad + \frac{1}{N^2} \sum_{i=1}^N \int_\potspace \sbr*{ 2 \br*{\sum_{j=1}^N \psi(X_r^j) - \psi(X_r^i)} (\psi(y) - \psi(X_r^i)) + \psi^2(y) - \psi^2(X_r^i) } \lambda \kappa(X_r^i,\odif{y}) \Bigg\} \odif{r} \\
    %
    \overset{\zcref{eq:kappa-to-mean-kappa}}&{=} \br*{ \int_\potspace \psi(x) \mu_t^{\lambda, N}(\odif{x}) }^2 - \br*{ \int_\potspace \psi(x) \mu_0^{\lambda, N}(\odif{x}) }^2 \\
    &\quad {} - \int_0^t \Bigg\{ 2 \int_\potspace \int_\potspace b(x) \psi(y) \partial_x \psi (x) \mu_r^{\lambda,N}(\odif{x}) \mu_r^{\lambda,N}(\odif{y}) \\
    &\quad + \frac{1}{N} \int_\potspace \int_\potspace \sbr*{ 2 (\psi(y) - \psi(x)) \br*{\sum_{j=1}^N \psi(X_r^j) - \psi(x)} + \psi^2(y) - \psi^2(x) } \lambda \ol{\kappa}_r(x,\odif{y}) \mu_r^{\lambda, N}(\odif{x}) \Bigg\} \odif{r} \\
    %
    \overset{(N\to\infty)}&{=} \br*{ \int_\potspace \psi(x) \mu_t^{\lambda, N}(\odif{x}) }^2 - \br*{ \int_\potspace \psi(x) \mu_0^{\lambda, N}(\odif{x}) }^2 - 2 \int_0^t \int_\potspace \int_\potspace \bigg\{ b(x) \psi(y) \partial_x \psi(x) \\
    &\quad + \int_\potspace (\psi(z) - \psi(x)) \psi(y) \lambda \ol{\kappa}_r(x,\odif{z}) \bigg\} \mu_{r}^{\lambda, N} (\odif{x}) \mu_{r}^{\lambda, N} (\odif{y}) \odif{r} + \mathcal{O}(N^{-1}) \\
    &= \br*{ \int_\potspace \psi \odif{\mu_t^{\lambda, N}} }^2 - \br*{ \int_\potspace \psi \odif{\mu_0^{\lambda, N}} }^2 - 2 \int_0^t \int_\potspace \psi(y) \mu_{r}^{\lambda, N} (\odif{y}) \int_\potspace \widehat{L}_r^{\lambda, N} [\psi](x) \mu_{r}^{\lambda, N} (\odif{x}) \odif{r} + \mathcal{O}(N^{-1}) \\
    &= S_t^2 - S_0^2 - 2 \int_0^t S_{r-} \odv{A_{r}}{r} \odif{r} + \mathcal{O}(N^{-1}) \\
    &= S_t^2 - S_0^2 - 2 \int_0^t S_{r-} \odif{A_{r}} + \mathcal{O}(N^{-1}) \\
    &= S_t^2 - S_0^2 - 2 \int_0^t S_{r-} \odif{\br*{S_{r} - S_0 - \widehat{M}_{r}^{\lambda,N}}} + \mathcal{O}(N^{-1}) \\
    &= S_t^2 - S_0^2 - 2 \int_0^t S_{r-} \odif{S_{r}} + 2 \int_0^t S_{r} \odif{\widehat{M}_{r}^{\lambda,N}} + \mathcal{O}(N^{-1}) \\
    \overset{\eqref{eq:S^2-q-var-rel}}&{=} \sbr{S}_t + 2 \int_0^t S_{r-} \odif{\widehat{M}_{r-}^{\lambda,N}} + \mathcal{O}(N^{-1}),
\end{split}
\end{equation}
Now, note that the first term equals $\sbr{\widehat{M}^{\lambda,N}}_t$ because $A$ is of bounded variation (so its quadratic variation is zero).
The second term is a martingale so it vanishes in expectation.
Hence
\begin{equation}
    \Var{\lawmu^{\lambda,N}}{\widehat{M}_t^{\lambda,N}}
    = \Exp{\lawmu^{\lambda,N}}{\sbr{\widehat{M}^{\lambda,N}}_t}
    = \Exp*{\lawmu^{\lambda,N}}{M_t^{\lambda, N}\sbr*{ \br*{ \frac{1}{N} \bigoplus_{i=1}^N \psi }^2 }} + \mathcal{O}(N^{-1})
    = \mathcal{O}(N^{-1}) \overset{N\to\infty}{\to} 0.
\end{equation}
\end{proof}


\begin{theorem}
    For fixed $\lambda > 0$, $\Set{ \lawmu^{\lambda, N} }_{N\in\bN} \subset \cP(D_{\cP(\potspace)}[0,T])$ is relatively compact.
    % \begin{equation}
    %     \operatorname{Law}(\mu^{\lambda, N}) = \lawmu^{\lambda, N} \wto \bar{\lawmu} \in \mathcal{P}(D_{\mathcal{P}(\potspace)}[0,T])
    % \end{equation}
    % as $N\to\infty$.
\end{theorem}

\begin{proof}
By Prokhorov's Theorem \cite[Theorem 5.1]{billingsley_convergence_1999}, it suffices to show that $\Set{ \lawmu^{\lambda, N} }_{N\in\bN}$ is tight.
Recall that $\lawmu^{\lambda, N}$ is the law of the empirical measure process $\mu^{\lambda, N}$.
Because $(\cP(\potspace), \pi)$ is a (complete, separable) metric space with $\pi$ the standard Prokhorov metric that metrizes weak convergence \cite[Theorem 6.8]{billingsley_convergence_1999}, Corollary 21 of Kouritzin \cite{kouritzin_tightness_2015} tells us that it suffices to show that the compact containment condition (CCC) and the weak modulus of continuity condition (WMCC) hold.

To verify the CCC we have to show that
\begin{equation}
    \forall \eps > 0 : \exists \cK_\eps \Subset \cP(\potspace) :
    \inf_{N\in\bN} P^{\lambda, N} (\mu_t^{\lambda, N} \in \cK_\eps,\ 0 \leq t \leq T) \geq 1 - \eps.
\end{equation}
Let $\eps > 0$, and simply define
\begin{equation}
    \cK_\eps \coloneqq \Set{ \mu_t^{\lambda, N} \given t \in [0,T],\  }
\end{equation}

% As $\potspace$ is compact, complete and separable, $\cP(\potspace)$ is compact w.r.t. the weak topology by Prokhorov's Theorem.
% Therefore, it is clear that the family of processes $\{\mu^{\lambda, N}\}_{N\in\bN} \subset \cP(\potspace)$ satisfies CCC.

\bigskip

To verify that the WMCC holds, we define the following collection of functions on $\cP(\potspace)$:
\begin{equation}
    \cG \coloneqq \Set{\nu \mapsto \int_\potspace \psi \odif{\nu} \given \psi \in C^1(\potspace) \cap C_0(\potspace)}.
\end{equation}
Because we are using the topology of weak convergence on $\cP(\potspace)$, it follows from $C^1(\potspace) \cap C_0(\potspace) \subset C_b(\potspace)$ that $\cG \subset C(\cP(\potspace))$.
Furthermore, $\cG$ is closed under addition and it separates points (on compacts).

Let $g = g_\psi \in \cG$.
It now suffices to show that $\{g \circ \mu^{\lambda, N}\}_{N\in\bN}$ satisfies the asymptotic modulus of continuity condition (AMCC).
Let $\eta > 0$.
% By taking $\mathcal{J} \coloneqq \{\Id\} \subset C_b(\cP(\potspace))$, which clearly strongly separates points, in Proposition 14 b)
Let $N_0 \in \bN$ such that $\Exp{}{[M_T^{\lambda, N}]} < $, which is possible by \zcref{prop:vanishing-variance}, and let $N \geq N_0$.
Now observe that
\begin{equation}
    g \circ \mu^{\lambda, N} = \int_\potspace \psi \odif{\mu^{\lambda, N}} = S^{\lambda, N} = M^{\lambda, N} - A^{\lambda, N}.
\end{equation}
It follows that for $C_\lambda^\psi \coloneqq \norm{b}_\infty \norm{\partial_x \psi}_\infty + 2\lambda \norm{\psi}_\infty$ (such that $\widehat{L}^{\lambda,N}_t [\psi] (x) \leq C_\lambda^\psi$ for all $t$, $x$) and $\delta \coloneqq \frac{1}{2C_\lambda^\psi}$ and a $\delta$-sparse partition $\{t_i\}$ such that $t_i - t_{i-1} < \frac{1}{C_\lambda^\psi}$, we have
\begin{equation}
\begin{split}
    P^{\lambda, N} (w'(g \circ \mu^{\lambda, N}, \delta) \geq \eta)
    &\leq P^{\lambda, N}( \max_i w(M^{\lambda, N}, [t_{i-1}, t_i)) + w(A^{\lambda, N}, [t_{i-1}, t_i) \geq \eta) \\
    &\leq P^{\lambda, N}( \max_i w(M^{\lambda, N}, [t_{i-1}, t_i)) \geq \frac{\eta}{2}) + P^{\lambda, N}(w(A^{\lambda, N}, [t_{i-1}, t_i) \geq \eta)
\end{split}
\end{equation}


% Since for any $\psi \in C_b(\potspace)$,
% \begin{equation}
%     \sup_{N\in\bN} \Exp{}{ \sup_{t\in[0,T]} \abs{ \int_\potspace \psi \odif{\mu_t^{\lambda,N}} } } \leq \norm{\psi}_{\infty},
% \end{equation}
% it suffices to show by the Aldous-Rebolledo criterion that both the martingale part and bounded variation part of $S_t$ have tight laws.
% For stopping times $0 \leq S \leq S' \leq S + \delta \leq T$, we have
% \begin{equation}
%     \Exp{}{ \widehat{M}_{S'}^{\lambda,N} - \widehat{M}_{S}^{\lambda,N} }
%     \overset{\text{(CS)}}{\leq} \Exp{}{ \abs{ \widehat{M}_{S'}^{\lambda,N} - \widehat{M}_{S}^{\lambda,N} }^2 }^{1/2}
%     \leq \Exp{}{\sbr{\widehat{M}^{\lambda,N}}_{S+\delta} - \sbr{\widehat{M}^{\lambda,N}}_{S}}^{1/2}
%     \overset{N\to\infty}{\to} 0
% \end{equation}
% by \zcref{prop:before}.
% The bounded variation part $A_{S'} - A_S$ also clearly goes to zero for $\delta \downarrow 0$.
\end{proof}


\printbibliography


% \begin{equation}
%     \mu^{\lambda, N} \coloneqq \frac{1}{N} \sum_{i=1}^N \delta_{X^i} \in \cP(\underbrace{D([0,T]; \potspace)}_{\eqqcolon \varGamma}),
%     \quad \mu_t^{\lambda, N} \coloneqq (e_t)_\# \mu^{\lambda, N},
%     \quad \varGamma \ni \omega \mapsto e_t(\omega) \coloneqq \omega_t.
% \end{equation}
% (Could see this as a push-forward of $P^{\lambda, N} \to (\Theta_N)_\# P^{\lambda, N}$ where $\Theta_N : \varGamma^N \to \cP(\varGamma); (\omega_1,\dots,\omega_N) \mapsto \frac{1}{N} \sum_{i=1}^N \delta_{\omega_i}$.)
% Let $P^{\lambda, N} \coloneqq \mathrm{Law}(\mu^{\lambda, N}) \in \cP(\cP(\varGamma))$.

% \begin{lemma}
%     If $\potspace$ is compact, the collection $\{P^{\lambda, N}\}_{\lambda,N}$ is tight.
% \end{lemma}
% \begin{proof}
%     Because $\potspace$ is compact, $W_1$ metrizes the narrow topology on $\cP(\varGamma)$.
%     We have for all $\omega \in \Omega$,
%     \begin{equation}
%         W_1(\mu^{\lambda, N}(\omega), \delta_0)
%         = \int_{\varGamma} d_\varGamma(\gamma,0) \mu^{\lambda,N}(\omega) (\odif{\gamma})
%         = \int_{\varGamma} \sup_{t \in [0,T]} \abs{\gamma_t} \mu^{\lambda,N}(\omega) (\odif{\gamma})
%         = \frac{1}{N} \sum_{i=1}^N \sup_{t \in [0,T]} \abs{X^i_t(\omega)} \leq C,
%     \end{equation}
%     for some $C > 0$.
%     Hence
%     \begin{equation}
%         \sup_{\lambda, N} \int_\Omega W_1(\mu^{\lambda, N}(\omega), \delta_0) P^{\lambda, N}(\odif{\omega})
%         = \Exp{}{W_1(\mu^{\lambda, N}, \delta_0)} < +\infty.
%     \end{equation}
%     By an OT exercise, this implies tightness.
% \end{proof}



% The martingale property is
% \begin{equation}
%     \Exp{}{M_t^{\lambda, N}[\varphi] - M_s^{\lambda, N}[\varphi] \given \cF_s} = 0
% \end{equation}
% for $\cF_t \coloneqq \sigma(X_s : s \leq t)$.


% I think we need, for Feller process:
% \begin{itemize}
%     \item A collection of probability measures $\{P^\bm{Z}, \bm{Z} \in \bR^N\}$ on $(D_\bR([0,T])^N, \cF)$;

%     \item A right-continuous filtration $\{\cF_t, t \geq 0\}$ on $D_\bR([0,T])^N$ with respect to which $\bm{X}_t$ is adapted, and
%     \begin{equation}
%         P^\bm{Z}(\bm{X}(0) = \bm{Z}) = 1,
%     \end{equation}
%     the mapping $x \mapsto E^\bm{Z} \varphi(\bm{X}_t)$ is in $C_0(\bR^N)$ for all $\varphi \in C_0(\bR^N)$ and $t \geq 0$,
%     and
%     \begin{equation}
%         E^\bm{Z}[ \bm{Y} \circ \theta_s \mid \cF_s] = E^{\bm{X}_s} \bm{Y} \quad \text{a.s. } P^\bm{Z}
%     \end{equation}
%     for all $\bm{Z} \in \bR^N$ and all bounded measurable $\bm{Y}$ on $D_\bR([0,T])^N$. Here $(\theta_s\omega)_t = \omega{t+s}$.
% \end{itemize}



\end{document}
